Pom/Lpo/Operations/Seq/Branches.lean
@@ -1,14 +1,27 @@
+import Pom.Lpo.Linearization.Label
 import Pom.Lpo.Order.FinApprox
 
 namespace Lpofin
 
-variable {l : Type} [PartialOrder l] [OrderBot l]
+variable {act test : Type}
+
+def isTest (α : Lpofin (Label act test)) (x : Node) : Prop := Label.isTest (α.lab x)
+
+def tests (α : Lpofin (Label act test)) : Set Node := { x | α.isTest x }
+
+lemma tests_sub_nodes {α : Lpofin (Label act test)} : α.tests ⊆ α.nodes := by
+  intro x hx
+  refine (α.val.property.lab_dom x).mt ?_ |> not_not.mp
+  have ⟨b, hlab⟩ := (Label.isTest_iff _).mp hx
+  conv => arg 1; lhs; exact hlab
+  exact Label.test_ne_bot _
 
 -- stuck is a path condition formula indicating that the execution will definitely
 -- encounter a ⊥ node
-def stuck (α : Lpofin l) : Form Node := Form.sOr fun x : ↑α.val.bots ↦ α.form x.val
+def stuck (α : Lpofin (Label act test)) : Form Node := Form.sOr fun x : ↑α.val.bots ↦ α.form x.val
 
-lemma stuck_antitone : @Antitone (Lpofin l) _ _ _ stuck := by
+lemma stuck_antitone [PartialOrder act] [PartialOrder test] :
+    @Antitone (Lpofin (Label act test)) _ _ _ stuck := by
   intro α β hle v ⟨⟨x, hx, hlab⟩, hform⟩
   rcases hle.succ _ hx with hx' | ⟨y, ⟨hy, hlab'⟩, hyx⟩
   · refine ⟨⟨x, hx', ?_⟩, ?_⟩
@@ -21,145 +34,87 @@ lemma stuck_antitone : @Antitone (Lpofin l) _ _ _ stuck := by
     refine (β.val.property.form _ (hle.nodes hy)).2 _ hyx _ ?_
     exact hform
 
--- A node is in the exntensible set if it is possible for it not be stuck
-def extens (α : Lpofin l) : Set Node :=
-  { x ∈ α.nodes | ¬ α.form x ≤ α.stuck }
-
-lemma extens_finite (α : Lpofin l) : α.extens.Finite := by
-  apply α.property.subset; intro x hx; exact hx.1
-
-lemma extens_not_bot {α : Lpofin l} {x : Node} : x ∈ α.extens → α.lab x ≠ ⊥ := by
-  intro h heq; apply h.2; intro v hform
-  refine ⟨⟨x, ?_, heq⟩, hform⟩
-  exact (α.val.property.form_dom x).mp ⟨v, hform⟩
-
-lemma extens_monotone : @Monotone (Lpofin l) _ _ _ extens := by
-  intro α β hle x ⟨hx, hstuck⟩
-  refine ⟨hle.nodes hx, ?_⟩; intro hc
-  refine hstuck (fun v hform ↦ stuck_antitone hle v (hc v ?_))
-  simp only [form]; rw [← hle.form x hx]; exact hform
-
-lemma le_extens {α β : Lpofin l} (hle : α ≤ β) :
-    α.extens = { x ∈ β.extens | ¬ (β.form x ≤ α.stuck) } := by
-  ext x; constructor
-  · intro hx; refine ⟨extens_monotone hle hx, ?_⟩
-    intro c; refine hx.2 (le_trans ?_ c)
-    exact le_form hle
-  · intro ⟨⟨hx, _⟩, hstk⟩
-    rcases hle.succ _  hx with hxα | ⟨y, ⟨hy, hbot⟩, hyx⟩
-    · refine ⟨hxα, ?_⟩
-      intro c; refine hstk (le_of_eq_of_le (Eq.symm ?_) c)
-      exact hle.form _ hxα
-    · exfalso; refine hstk (((β.val.property.form y (hle.nodes hy)).2 _ hyx).trans ?_)
-      refine le_of_eq_of_le (Eq.symm (hle.form _ hy)) ?_
-      intro v hform; exact ⟨⟨y, hy, hbot⟩, hform⟩
-
-def conj (α : Lpofin l) (S : Set Node) : Form Node :=
+def conj (α : Lpofin (Label act test)) (S : Set Node) : Form Node :=
   Form.sAnd fun x : ↑S ↦ α.form x.val
 
-def branches (α : Lpofin l) : Set (Form Node) :=
-  α.conj ''
-  { S : Set Node
-  | S.Nonempty ∧
-    S ⊆ α.extens ∧
-    (α.conj S).sat ∧
-    α.conj S ≤ α.stuck.not ∧
-    ∀ T, S ⊂ T → T ⊆ α.extens → ¬ Form.sat (fun v ↦ ∀ x ∈ T, α.form x v)
+def node_lit (x : Node) (b : Bool) : Form Node :=
+  if b then Form.literal x else (Form.literal x).not
+
+lemma node_lit_depends_on {x : Node} {b : Bool} : Form.DependsOn (node_lit x b) {x} := by
+  cases b
+  · exact Form.DependsOn.literal.not
+  · exact Form.DependsOn.literal
+
+def mk_form {t : Set Node} (f : ↑t → Bool) : Form Node :=
+  Form.sAnd (fun x ↦ node_lit x.val (f x))
+
+lemma mk_form_depends_on {t : Set Node} (f : ↑t → Bool) : Form.DependsOn (mk_form f) t := by
+  conv => arg 2; exact (Set.iUnion_of_singleton_coe t).symm
+  refine Form.DependsOn.sAnd fun _ ↦ node_lit_depends_on
+
+def reachable (α : Lpofin (Label act test)) (t : Set Node) (f : ↑t → Bool) : Prop :=
+  (mk_form f).sat ∧
+  mk_form f ≤ α.conj t ∧
+  mk_form f ≤ α.stuck.not
+
+def branches (α : Lpofin (Label act test)) : Set (Form Node) :=
+  { φ : Form Node
+  | ∃ t ⊆ α.tests,
+    ∃ f : ↑t → Bool,
+      φ = mk_form f ∧
+      reachable α t f ∧
+      ∀ {x b}, x ∉ t → α.isTest x →
+        ¬ α.reachable (insert x t)
+          fun ⟨z, hz⟩ ↦ if h : z = x then b else f ⟨z, Set.mem_of_mem_insert_of_ne hz h⟩
   }
 
-lemma branches_finite (α : Lpofin l) : α.branches.Finite := by
-  refine Set.Finite.image _ ?_
-  refine α.extens_finite.powerset.subset ?_
-  intro s ⟨_, hsub, _⟩; exact hsub
+lemma branches_finite (α : Lpofin (Label act test)) : α.branches.Finite := by
+  sorry
 
-lemma branches_monotone : @Monotone (Lpofin l) _ _ _ branches := by
-  classical
-  rintro α β hle φ ⟨S, ⟨hne, hsub, hsat, hstuck, hmax⟩, hφ⟩; subst hφ
-  refine ⟨S, ⟨hne, ?_, ?_, ?_, ?_⟩, ?_⟩
-  · exact le_trans hsub (extens_monotone hle)
-  · rcases hsat with ⟨v, hv⟩; use v; intro x
-    refine (congrFun (hle.form x ?_) _).mp (hv x)
-    exact hsub x.property |>.1
-  · intro v hform hstuck'; refine hstuck v ?_ ?_
-    · intro x; refine (congr_fun (hle.form x ?_) v).mpr (hform x)
-      exact hsub x.property |>.1
-    · exact stuck_antitone hle v hstuck'
-  · intro T hST hT ⟨v, hc⟩; obtain ⟨x, hxT, hxS⟩ := Set.exists_of_ssubset hST
-    have hform : α.conj S v := by
-      intro y; refine (congrFun (hle.form _ ?_) _).mpr (hc _ ?_)
-      · exact (hsub y.property).1
-      · exact hST.subset y.property
-    rcases hle.succ _ (hT hxT).1
-      with hx | ⟨y, hy, hyx⟩
-    · refine hmax (insert x S) (Set.ssubset_insert hxS) ?_ ?_
-      · refine Set.insert_subset ⟨hx, ?_⟩ hsub
-        · intro c; refine hstuck v hform ?_
-          exact c v ((congrFun (hle.form _ hx) _).mpr (hc _ hxT))
-      · use v; intro y hy; rcases Set.mem_insert_iff.mp hy with rfl | hy'
-        · exact (congrFun (hle.form y hx) _).mpr (hc y hxT)
-        · refine (congrFun (hle.form y ?_) _).mpr (hc y ?_)
-          · exact (hsub hy').1
-          · exact hST.subset hy'
-    · refine hstuck v hform ⟨⟨y, hy⟩, ?_⟩
-      refine (congrFun (hle.form _ hy.1) _).mpr ?_
-      exact (β.val.property.form _ (hle.nodes hy.1)).2 _ hyx v (hc _ hxT)
-  · ext1 v; refine forall_congr fun x ↦ ?_; ext; constructor
-    · intro h; refine (congr_fun (hle.form x ?_) v).mpr h
-      exact (hsub x.property).1
-    · intro h; refine (congr_fun (hle.form x ?_) v).mp h
-      exact (hsub x.property).1
+lemma branches_monotone [PartialOrder act] [PartialOrder test] :
+    @Monotone (Lpofin (Label act test)) _ _ _ branches := by
+  rintro α β hle φ ⟨t, ht, f, rfl, ⟨⟨v, hform⟩, himp, hstk⟩, hmax⟩
+  refine ⟨t, ?_, f, rfl, ?_, ?_⟩
+  · intro x hx
+    have ⟨b, heq⟩ := (Label.isTest_iff _).mp (ht hx)
+    apply (Label.isTest_iff _).mpr
+    have hlab := le_of_eq_of_le heq.symm <| hle.lab x
+    have ⟨b', hb, _⟩ := lab_is_test_le hlab; exact ⟨b', hb⟩
+  · refine ⟨⟨v, hform⟩, ?_, ?_⟩
+    · intro v hv x; exact le_form hle v (himp _ hv x)
+    · intro v hf h; apply hstk v hf
+      exact stuck_antitone hle _ h
+  · sorry
 
-lemma le_branches {α β : Lpofin l} (hle : α ≤ β) :
+lemma le_branches [PartialOrder act] [PartialOrder test] {α β : Lpofin (Label act test)} (hle : α ≤ β) :
     α.branches = { φ ∈ β.branches | φ ≤ α.stuck.not } := by
   ext φ; constructor
   · intro h; constructor
     · exact branches_monotone hle h
-    · rcases h with ⟨_, ⟨_, _, _, hstuck, _⟩, rfl⟩
+    · obtain ⟨_, _, _, rfl, ⟨_, _, hstuck⟩, _⟩ := h
       exact hstuck
-  · rintro ⟨⟨S, ⟨hne, hsub, ⟨v, hsat⟩, _, hmax⟩, rfl⟩, hstuck⟩
-    have hS x (hx : x ∈ S) : x ∈ α.nodes := by
-      rcases hle.succ _ (hsub hx).1 with hxα | ⟨y, hbot, hyx⟩
+  · rintro ⟨⟨t, ht, f, rfl, ⟨⟨v, hsat⟩, himp, _⟩, hmax⟩, hstuck⟩
+    have hsub : t ⊆ α.nodes := by
+      intro x hxt
+      have hx := tests_sub_nodes <| ht hxt
+      rcases hle.succ _ hx with hxα | ⟨y, hbot, hyx⟩
       · exact hxα
       · exfalso; refine forall_not_of_not_exists (hstuck v hsat) ⟨y, hbot⟩ ?_
         refine (congrFun (hle.form y hbot.1) _).mpr ?_
         refine (β.val.property.form y (hle.nodes hbot.1)).2 _ hyx v ?_
-        exact hsat ⟨_, hx⟩
-    refine ⟨S, ⟨hne, ?_, ⟨v, ?_⟩, ?_, ?_⟩, ?_⟩
-    · intro x hx; rw [le_extens hle]
-      refine ⟨hsub hx, ?_⟩
-      intro c; exact hstuck v hsat (c v (hsat ⟨x, hx⟩))
-    · intro x; exact (congrFun (hle.form x (hS _ x.property)) _).mpr (hsat x)
-    · refine le_trans ?_ hstuck; intro u hu x
-      exact (congrFun (hle.form _ (hS _ x.property)) _).mp (hu x)
-    · intro T hST hT ⟨u, hu⟩; refine hmax T hST ?_ ?_
-      · exact le_trans hT (extens_monotone hle)
-      · use u; intro x hx; refine (congrFun (hle.form _ ?_) _).mp (hu _ hx)
-        exact (hT hx).1
-    · ext1 u; refine forall_congr fun x ↦ ?_
-      exact congrFun (hle.form x (hS _ x.property)) _
+        exact himp _ hsat ⟨_, hxt⟩
+    refine ⟨t, ?_, f, rfl, ⟨⟨v, hsat⟩, ?_, hstuck⟩, ?_⟩
+    · intro x hx; sorry
+    · intro v hform x; have hx := hsub x.property
+      exact (congrFun (hle.form _ hx) _).mpr (himp _ hform x)
+    · intro x b hx htst; sorry
 
-lemma branches_not_mutually_sat {α : Lpofin l} {φ ψ : Form Node}
+lemma branches_not_mutually_sat {α : Lpofin (Label act test)} {φ ψ : Form Node}
     (hφ : φ ∈ α.branches) (hψ : ψ ∈ α.branches) (hneq : φ ≠ ψ) :
     ∀ v, ¬ (φ v ∧ ψ v) := by
   intro v ⟨h₁, h₂⟩
-  obtain ⟨S, ⟨_, hsub, _, _, hmax⟩, rfl⟩ := hφ
-  obtain ⟨T, ⟨_, hsub', _, _, hmax'⟩, rfl⟩ := hψ
-  refine hmax (S ∪ T) ⟨Set.subset_union_left, ?_⟩ ?_ ?_
-  · intro h; apply hneq; refine congrArg _ ?_; ext x; constructor
-    · intro hx; by_contra ht; refine hmax' (insert x T) ?_ ?_ ?_
-      · exact Set.ssubset_insert ht
-      · intro y hy; rcases Set.mem_insert_iff.mp hy with rfl | hy
-        · exact hsub hx
-        · exact hsub' hy
-      · use v; intro y hy; rcases Set.mem_insert_iff.mp hy with rfl | hy
-        · exact h₁ ⟨y, hx⟩
-        · exact h₂ ⟨y, hy⟩
-    · intro hx; exact h (Set.subset_union_right hx)
-  · rintro x (hx | hx)
-    · exact hsub hx
-    · exact hsub' hx
-  · use v; rintro x (hx | hx)
-    · exact h₁ ⟨x, hx⟩
-    · exact h₂ ⟨x, hx⟩
+  obtain ⟨t, ht, f, rfl, hr, hmax⟩ := hφ
+  obtain ⟨u, hu, g, rfl, hr', hmax'⟩ := hψ
+  sorry
 
 end Lpofin
